a bit of clean-up

src/canonize/tactic.lean
@@ -1,5 +1,5 @@
 import data.list.alist data.finmap
-import .sterm .pterm
+import .norm
 
 namespace list
 open tactic
@@ -79,164 +79,6 @@ begin
 end
 
 end eterm
-
-inductive alt {γ} [const_space γ] : Type
-| sform : list (@nterm γ _) → @sterm γ _ → alt
-| pform : list (@nterm γ _) → @pterm γ _ → alt
-
-namespace alt
-open nterm
-
-variables {α : Type} [discrete_field α]
-variables {γ : Type} [const_space γ]
-variables [morph γ α] {ρ : dict α}
-
-def singleton (x : @nterm γ _) : @alt γ _ :=
-sform [] (sterm.singleton x)
-
-def to_nterm : @alt γ _ → @nterm γ _
-| (sform _ S) := S.to_nterm
-| (pform _ P) := P.to_nterm
-
-def hyps : @alt γ _ → list (@nterm γ _)
-| (sform l _) := l
-| (pform l _) := l
-
-def eval (ρ : dict α) (x : @alt γ _) : α :=
-nterm.eval ρ x.to_nterm
-
-theorem eval_def {x : @alt γ _} : eval ρ x = nterm.eval ρ x.to_nterm := rfl
-
-def reduce : @alt γ _ → @alt γ _
-| (sform l S) := sform l S.reduce
-| (pform l P) := pform (l ∪ P.reduce_hyps) P.reduce
-
-def reduce_hyps : @alt γ _ → list (@nterm γ _)
-| (sform l S) := []
-| (pform l P) := P.reduce_hyps
-
-def to_sterm : @alt γ _ → @sterm γ _
-| (sform _ S) := S
-| x := sterm.of_nterm x.to_nterm
-
-def to_pterm : @alt γ _ → @pterm γ _
-| (pform _ P) := P
-| x := pterm.of_nterm x.to_nterm
-
-theorem eval_singleton {x : @nterm γ _} :
-  eval ρ (singleton x) = nterm.eval ρ x :=
-begin
-  unfold singleton, unfold eval, unfold to_nterm,
-  rw [← sterm.eval_to_nterm, sterm.eval_singleton]
-end
-
-theorem eval_reduce {x : @alt γ _} :
-  nonzero ρ x.reduce_hyps →
-  eval ρ x.reduce = eval ρ x :=
-begin
-  intro H,
-  cases x with l S l P,
-  { unfold reduce, unfold eval, unfold to_nterm,
-    rw [← sterm.eval_to_nterm, ← sterm.eval_reduce, sterm.eval_to_nterm] },
-  { unfold reduce, unfold eval, unfold to_nterm,
-    rw [← pterm.eval_to_nterm, ← pterm.eval_reduce H, pterm.eval_to_nterm] }
-end
-
-theorem eval_to_sterm {x : @alt γ _} :
-  eval ρ x = sterm.eval ρ x.to_sterm :=
-begin
-  cases x,
-  { unfold to_sterm, unfold eval, unfold to_nterm, rw ← sterm.eval_to_nterm },
-  { unfold to_sterm, unfold eval, unfold to_nterm, rw ← sterm.eval_of_nterm }
-end
-
-theorem eval_to_pterm {x : @alt γ _} :
-  eval ρ x = pterm.eval ρ x.to_pterm :=
-begin
-  cases x,
-  { unfold to_pterm, unfold eval, unfold to_nterm, rw ← pterm.eval_of_nterm },
-  { unfold to_pterm, unfold eval, unfold to_nterm, rw ← pterm.eval_to_nterm }
-end
-
-def add (x y : @alt γ _) : @alt γ _ :=
-sform (x.hyps ∪ y.hyps) (x.to_sterm + y.to_sterm)
---TODO: more cases to avoid switching form too often
-
-def mul (x y : @alt γ _) : @alt γ _ :=
-pform (x.hyps ∪ y.hyps) (x.to_pterm * y.to_pterm)
---TODO: more cases to avoid switching form too often
-
-def pow (x : @alt γ _) (n : znum) : @alt γ _ :=
-if n = 0 then singleton (1 : γ)
-else if n = 1 then x
-else pform x.hyps (x.to_pterm ^ n)
-
-instance : has_add (@alt γ _) := ⟨add⟩
-instance : has_mul (@alt γ _) := ⟨mul⟩
-instance : has_pow (@alt γ _) znum := ⟨pow⟩
-
-@[simp] theorem hyps_add {x y : @alt γ _} :
-  (x + y).hyps = x.hyps ∪ y.hyps :=
-by { simp [hyps, has_add.add, add] }
-
-@[simp] theorem hyps_mul {x y : @alt γ _} :
-  (x * y).hyps = x.hyps ∪ y.hyps :=
-by { simp [hyps, has_mul.mul, mul] }
-
-@[simp] theorem hyps_pow {x : @alt γ _} {n : znum} :
-  (x ^ n).hyps = if n = 0 then [] else x.hyps :=
-begin
-  by_cases h0 : n = 0;
-  by_cases h1 : n = 1;
-  simp [h0, h1, has_pow.pow, pow, hyps, singleton]
-end
-
-def of_nterm : @nterm γ _ → @alt γ _
-| (nterm.add x y) := of_nterm x + of_nterm y
-| (nterm.mul x y) := of_nterm x * of_nterm y
-| (nterm.pow x n) := of_nterm x ^ n
-| x := singleton x
-
-theorem eval_of_nterm {x : @nterm γ _} :
-  nonzero ρ (of_nterm x).hyps →
-  eval ρ (of_nterm x) = nterm.eval ρ x :=
-begin
-  induction x with i c x y ihx ihy x y ihx ihy x n ihx,
-  { intro, unfold of_nterm, rw eval_singleton },
-  { intro, unfold of_nterm, rw eval_singleton },
-  repeat {sorry}
-end
-
-end alt
-
-namespace nterm
-
-variables {α : Type} [discrete_field α]
-variables {γ : Type} [const_space γ]
-variables [morph γ α] {ρ : dict α}
-
-def naive_norm : @nterm γ _ → @nterm γ _
-| (add x y) := (sterm.of_nterm (naive_norm x) + sterm.of_nterm (naive_norm y)).reduce.to_nterm
-| (mul x y) := (pterm.of_nterm (naive_norm x) * pterm.of_nterm (naive_norm y)).reduce.to_nterm
-| (pow x n) := (pterm.of_nterm (naive_norm x) ^ n).reduce.to_nterm
-| x := x
-
-def norm (x : @nterm γ _) : @nterm γ _ := (alt.of_nterm x).to_nterm
-def norm_hyps (x : @nterm γ _) : list (@nterm γ _) := (alt.of_nterm x).hyps
-
-theorem soundness {x : @nterm γ _} :
-  norm x = naive_norm x :=
-by sorry
-
-def correctness {x : @nterm γ _} :
-  nonzero ρ (norm_hyps x) →
-  nterm.eval ρ x = nterm.eval ρ (norm x) :=
-begin
-  sorry
-end
-
-end nterm
-
 open eterm native tactic
 
 meta structure cache_ty :=
@@ -263,7 +105,6 @@ end
 def list_to_dict {α} [inhabited α] (l : list α) : dict α :=
 ⟨λ i, list.func.get i l⟩
 
-
 def finmap.to_dict (m : finmap (λ _ : num, ℝ)) : dict ℝ :=
 ⟨λ i, match finmap.lookup i m with (some x) := x | _ := 0 end⟩
 
@@ -282,6 +123,7 @@ do
 
 @[reducible]
 def γ := ℚ
+--TODO: replace with Qnum
 
 instance : const_space γ :=
 { df := by apply_instance,
@@ -347,21 +189,6 @@ match e with
 | _ := atom <$> get_atom e
 end
 
-meta def nterm_to_expr (f : num → expr) : @nterm γ _ → tactic expr
-| (nterm.atom i)  := return (f i)
-| (nterm.const c) := to_expr ``(%%(reflect c) : ℝ)
-| (nterm.add x y) := do
-  a ← nterm_to_expr x,
-  b ← nterm_to_expr y,
-  to_expr ``(%%a + %%b)
-| (nterm.mul x y) := do
-  a ← nterm_to_expr x,
-  b ← nterm_to_expr y,
-  to_expr ``(%%a * %%b)
-| (nterm.pow x n) := do
-  a ← nterm_to_expr x,
-  to_expr ``(%%a ^ (%%(reflect n) : ℤ))
-
 def norm (x : @eterm γ _) : @nterm γ _ :=
 x.to_nterm.norm
 
@@ -378,6 +205,21 @@ begin
   { apply eterm.correctness },
   { apply nterm.correctness H }
 end
+
+meta def nterm_to_expr (f : num → expr) : @nterm γ _ → tactic expr
+| (nterm.atom i)  := return (f i)
+| (nterm.const c) := to_expr ``(%%(reflect c) : ℝ)
+| (nterm.add x y) := do
+  a ← nterm_to_expr x,
+  b ← nterm_to_expr y,
+  to_expr ``(%%a + %%b)
+| (nterm.mul x y) := do
+  a ← nterm_to_expr x,
+  b ← nterm_to_expr y,
+  to_expr ``(%%a * %%b)
+| (nterm.pow x n) := do
+  a ← nterm_to_expr x,
+  to_expr ``(%%a ^ (%%(reflect n) : ℤ))
 
 meta def norm_expr (e : expr) : tactic (@nterm γ _ × expr × expr) :=
 do
