src/canonize/norm.lean
@@ -1,0 +1,167 @@
+import .sterm .pterm
+
+namespace polya
+
+inductive alt {γ} [const_space γ] : Type
+| sform : list (@nterm γ _) → @sterm γ _ → alt
+| pform : list (@nterm γ _) → @pterm γ _ → alt
+
+namespace alt
+open nterm
+
+variables {α : Type} [discrete_field α]
+variables {γ : Type} [const_space γ]
+variables [morph γ α] {ρ : dict α}
+
+def singleton (x : @nterm γ _) : @alt γ _ :=
+sform [] (sterm.singleton x)
+
+def to_nterm : @alt γ _ → @nterm γ _
+| (sform _ S) := S.to_nterm
+| (pform _ P) := P.to_nterm
+
+def hyps : @alt γ _ → list (@nterm γ _)
+| (sform l _) := l
+| (pform l _) := l
+
+def eval (ρ : dict α) (x : @alt γ _) : α :=
+nterm.eval ρ x.to_nterm
+
+theorem eval_def {x : @alt γ _} : eval ρ x = nterm.eval ρ x.to_nterm := rfl
+
+def reduce : @alt γ _ → @alt γ _
+| (sform l S) := sform l S.reduce
+| (pform l P) := pform (l ∪ P.reduce_hyps) P.reduce
+
+def reduce_hyps : @alt γ _ → list (@nterm γ _)
+| (sform l S) := []
+| (pform l P) := P.reduce_hyps
+
+def to_sterm : @alt γ _ → @sterm γ _
+| (sform _ S) := S
+| x := sterm.of_nterm x.to_nterm
+
+def to_pterm : @alt γ _ → @pterm γ _
+| (pform _ P) := P
+| x := pterm.of_nterm x.to_nterm
+
+theorem eval_singleton {x : @nterm γ _} :
+  eval ρ (singleton x) = nterm.eval ρ x :=
+begin
+  unfold singleton, unfold eval, unfold to_nterm,
+  rw [← sterm.eval_to_nterm, sterm.eval_singleton]
+end
+
+theorem eval_reduce {x : @alt γ _} :
+  nonzero ρ x.reduce_hyps →
+  eval ρ x.reduce = eval ρ x :=
+begin
+  intro H,
+  cases x with l S l P,
+  { unfold reduce, unfold eval, unfold to_nterm,
+    rw [← sterm.eval_to_nterm, ← sterm.eval_reduce, sterm.eval_to_nterm] },
+  { unfold reduce, unfold eval, unfold to_nterm,
+    rw [← pterm.eval_to_nterm, ← pterm.eval_reduce H, pterm.eval_to_nterm] }
+end
+
+theorem eval_to_sterm {x : @alt γ _} :
+  eval ρ x = sterm.eval ρ x.to_sterm :=
+begin
+  cases x,
+  { unfold to_sterm, unfold eval, unfold to_nterm, rw ← sterm.eval_to_nterm },
+  { unfold to_sterm, unfold eval, unfold to_nterm, rw ← sterm.eval_of_nterm }
+end
+
+theorem eval_to_pterm {x : @alt γ _} :
+  eval ρ x = pterm.eval ρ x.to_pterm :=
+begin
+  cases x,
+  { unfold to_pterm, unfold eval, unfold to_nterm, rw ← pterm.eval_of_nterm },
+  { unfold to_pterm, unfold eval, unfold to_nterm, rw ← pterm.eval_to_nterm }
+end
+
+def add (x y : @alt γ _) : @alt γ _ :=
+sform (x.hyps ∪ y.hyps) (x.to_sterm + y.to_sterm)
+--TODO: more cases to avoid switching form too often
+
+def mul (x y : @alt γ _) : @alt γ _ :=
+pform (x.hyps ∪ y.hyps) (x.to_pterm * y.to_pterm)
+--TODO: more cases to avoid switching form too often
+
+def pow (x : @alt γ _) (n : znum) : @alt γ _ :=
+if n = 0 then singleton (1 : γ)
+else if n = 1 then x
+else pform x.hyps (x.to_pterm ^ n)
+
+instance : has_add (@alt γ _) := ⟨add⟩
+instance : has_mul (@alt γ _) := ⟨mul⟩
+instance : has_pow (@alt γ _) znum := ⟨pow⟩
+
+@[simp] theorem hyps_add {x y : @alt γ _} :
+  (x + y).hyps = x.hyps ∪ y.hyps :=
+by { simp [hyps, has_add.add, add] }
+
+@[simp] theorem hyps_mul {x y : @alt γ _} :
+  (x * y).hyps = x.hyps ∪ y.hyps :=
+by { simp [hyps, has_mul.mul, mul] }
+
+@[simp] theorem hyps_pow {x : @alt γ _} {n : znum} :
+  (x ^ n).hyps = if n = 0 then [] else x.hyps :=
+begin
+  by_cases h0 : n = 0;
+  by_cases h1 : n = 1;
+  simp [h0, h1, has_pow.pow, pow, hyps, singleton]
+end
+
+def of_nterm : @nterm γ _ → @alt γ _
+| (nterm.add x y) := of_nterm x + of_nterm y
+| (nterm.mul x y) := of_nterm x * of_nterm y
+| (nterm.pow x n) := of_nterm x ^ n
+| x := singleton x
+
+theorem eval_of_nterm {x : @nterm γ _} :
+  nonzero ρ (of_nterm x).hyps →
+  eval ρ (of_nterm x) = nterm.eval ρ x :=
+begin
+  induction x with i c x y ihx ihy x y ihx ihy x n ihx,
+  { intro, unfold of_nterm, rw eval_singleton },
+  { intro, unfold of_nterm, rw eval_singleton },
+  repeat {sorry}
+end
+
+end alt
+
+namespace nterm
+
+variables {α : Type} [discrete_field α]
+variables {γ : Type} [const_space γ]
+variables [morph γ α] {ρ : dict α}
+
+def norm (x : @nterm γ _) : @nterm γ _ :=
+(alt.of_nterm x).to_nterm
+
+def norm_hyps (x : @nterm γ _) : list (@nterm γ _) :=
+(alt.of_nterm x).hyps
+
+def correctness {x : @nterm γ _} :
+  nonzero ρ (norm_hyps x) →
+  nterm.eval ρ x = nterm.eval ρ (norm x) :=
+begin
+  sorry
+end
+
+def naive_norm : @nterm γ _ → @nterm γ _
+| (add x y) := (sterm.of_nterm (naive_norm x) + sterm.of_nterm (naive_norm y)).reduce.to_nterm
+| (mul x y) := (pterm.of_nterm (naive_norm x) * pterm.of_nterm (naive_norm y)).reduce.to_nterm
+| (pow x n) := (pterm.of_nterm (naive_norm x) ^ n).reduce.to_nterm
+| x := x
+
+theorem soundness {x : @nterm γ _} :
+  norm x = naive_norm x :=
+begin
+  sorry
+end
+
+end nterm
+
+end polya
